theories/lang/cpp/logic/new_delete.v
@@ -54,17 +54,19 @@ Module Type Expr__newdelete.
     Context `{Σ : cpp_logic thread_info}.
 
     Section with_resolve.
-      Context {resolve:genv}.
-      Variables (ρ : region).
+      Context {σ : genv} (ρ : region).
+      Variable (tu : translation_unit).
 
-      #[local] Notation wp_prval := (wp_prval ρ).
-      #[local] Notation wp_init := (wp_init ρ).
-      #[local] Notation wp_initialize := (wp_initialize ρ).
-      #[local] Notation wp_operand := (wp_operand ρ).
-      #[local] Notation wp_args := (wp_args ρ).
-      #[local] Notation fspec := (fspec resolve.(genv_tu).(globals)).
+      #[local] Notation wp_prval := (wp_prval tu ρ).
+      #[local] Notation wp_init := (wp_init tu ρ).
+      #[local] Notation wp_initialize := (wp_initialize tu ρ).
+      #[local] Notation default_initialize := (default_initialize tu).
+      #[local] Notation wp_operand := (wp_operand tu ρ).
+      #[local] Notation wp_args := (wp_args tu ρ).
+      #[local] Notation interp := (interp tu).
+      #[local] Notation fspec := (fspec tu.(globals)).
 
-      #[local] Notation size_of := (@size_of resolve) (only parsing).
+      #[local] Notation size_of := (@size_of σ) (only parsing).
 
       #[local] Notation Tsize_t := Tu64 (only parsing).
       #[local] Notation Tbyte := Tuchar (only parsing).
@@ -122,7 +124,7 @@ Module Type Expr__newdelete.
             new_fn new_args aty Q targs sz
             (nfty := normalize_type new_fn.2)
             (_ : arg_types nfty = Some (Tnum sz Unsigned :: targs, Ar_Definite)),
-            wp_args (targs, Ar_Definite) new_args (fun vs free =>
+            wp_args  (targs, Ar_Definite) new_args (fun vs free =>
                 Exists sz al, [| size_of aty = Some sz |] ** [| has_type sz Tsize_t |] ** [| align_of aty = Some al |] **
                 Reduce (alloc_size_t sz (fun p FR =>
                 |> fspec nfty (_global new_fn.1) (p :: vs) (fun res => FR $
@@ -262,7 +264,7 @@ Module Type Expr__newdelete.
           in
           match erase_qualifiers ty with
           | Tnamed nm =>
-            match resolve.(genv_tu) !! nm with
+            match tu !! nm with
             | Some (Gstruct s) =>
               del $ from_option (fun x => (x, del_type)) default s.(s_delete)
             | Some (Gunion u) =>
@@ -287,7 +289,7 @@ Module Type Expr__newdelete.
           match drop_qualifiers ty with
           | Tqualified _ ty => False (* unreachable *)
           | Tnamed cls      =>
-            match resolve.(genv_tu) !! cls with
+            match tu !! cls with
             | Some (Gstruct s) =>
               if has_virtual_dtor s then
                 (* NOTE [has_virtual_dtor] could be derived from the vtable... *)
@@ -360,7 +362,7 @@ Module Type Expr__newdelete.
                (* v---- Calling destructor with object pointer *)
                resolve_dtor destroyed_type obj_ptr (fun this' mdc_ty =>
                     this' |-> new_tokenR mdc_ty **
-                    (destroy_val mdc_ty this' $
+                    (destroy_val tu mdc_ty this' $
                     Exists storage_ptr sz, [| size_of mdc_ty = Some sz |] **
                       (* v---- Token for converting obj memory to storage memory *)
                       provides_storage storage_ptr this' mdc_ty **
@@ -395,7 +397,7 @@ Module Type Expr__newdelete.
                obj_ptr |-> new_tokenR array_ty **
                (* /---- Calling destructor with object pointer
                   v     Note: virtual dispatch is not allowed for [delete[]] *)
-               destroy_val array_ty obj_ptr (
+               destroy_val tu array_ty obj_ptr (
                     Exists storage_ptr (sz sz' : N),
                       [| size_of array_ty = Some sz |] **
                       (* v---- Token for converting obj memory to storage memory *)
