theories/lang/cpp/logic/pred.v
@@ -261,17 +261,17 @@ Module Type CPP_LOGIC
       note that in the presence of code-loading, function calls will
       require an extra side-condition that the code is loaded.
      *)
-    Parameter code_at : genv -> Func -> ptr -> mpred.
-    Parameter method_at : genv -> Method -> ptr -> mpred.
-    Parameter ctor_at : genv -> Ctor -> ptr -> mpred.
-    Parameter dtor_at : genv -> Dtor -> ptr -> mpred.
+    Parameter code_at : genv -> translation_unit -> Func -> ptr -> mpred.
+    Parameter method_at : genv -> translation_unit -> Method -> ptr -> mpred.
+    Parameter ctor_at : genv -> translation_unit -> Ctor -> ptr -> mpred.
+    Parameter dtor_at : genv -> translation_unit -> Dtor -> ptr -> mpred.
 
     Section with_genv.
-      Context {σ : genv}.
-      Local Notation code_at := (code_at σ) (only parsing).
-      Local Notation method_at := (method_at σ) (only parsing).
-      Local Notation ctor_at := (ctor_at σ) (only parsing).
-      Local Notation dtor_at := (dtor_at σ) (only parsing).
+      Context {σ : genv} (tu : translation_unit).
+      #[local] Notation code_at := (code_at σ tu) (only parsing).
+      #[local] Notation method_at := (method_at σ tu) (only parsing).
+      #[local] Notation ctor_at := (ctor_at σ tu) (only parsing).
+      #[local] Notation dtor_at := (dtor_at σ tu) (only parsing).
 
       Axiom code_at_persistent : forall f p, Persistent (code_at f p).
       Axiom code_at_affine : forall f p, Affine (code_at f p).
@@ -708,15 +708,15 @@ Export L.
 Declare Module Export VALID_PTR : VALID_PTR_AXIOMS PTRS_INTF_AXIOM VALUES_INTF_AXIOM LC L.
 
 Section valid_ptr_code.
-  Context `{Σ : cpp_logic} {σ : genv}.
+  Context `{Σ : cpp_logic} {σ : genv} (tu : translation_unit).
 
-  Lemma code_at_valid   : forall f p,   code_at _ f p |-- valid_ptr p.
+  Lemma code_at_valid   : forall f p,   code_at _ tu f p |-- valid_ptr p.
   Proof. intros. rewrite code_at_strict_valid; apply strict_valid_valid. Qed.
-  Lemma method_at_valid : forall f p, method_at _ f p |-- valid_ptr p.
+  Lemma method_at_valid : forall f p, method_at _ tu f p |-- valid_ptr p.
   Proof. intros. rewrite method_at_strict_valid; apply strict_valid_valid. Qed.
-  Lemma ctor_at_valid   : forall f p,   ctor_at _ f p |-- valid_ptr p.
+  Lemma ctor_at_valid   : forall f p,   ctor_at _ tu f p |-- valid_ptr p.
   Proof. intros. rewrite ctor_at_strict_valid; apply strict_valid_valid. Qed.
-  Lemma dtor_at_valid   : forall f p,   dtor_at _ f p |-- valid_ptr p.
+  Lemma dtor_at_valid   : forall f p,   dtor_at _ tu f p |-- valid_ptr p.
   Proof. intros. rewrite dtor_at_strict_valid; apply strict_valid_valid. Qed.
 End valid_ptr_code.
 
